pulse/lib/pulse/core/PulseCore.IndirectionTheoryActions.fsti
@@ -68,11 +68,18 @@ val dup_inv (e:inames) (i:iref) (p:slprop)
     (inv i p) 
     (fun _ -> inv i p `star` inv i p)
 
-val fresh_invariant (e:inames) (p:slprop) (ctx:FStar.Ghost.erased (list iref))
-: ghost_act (i:iref{fresh_wrt ctx i}) e p (fun i -> inv i p)
+val fresh_invariant (e:inames) (p:slprop) (ctx:inames)
+: ghost_act
+   (i:iref{~(GhostSet.mem i ctx)})
+   e
+   (p `star` inames_live ctx)
+   (fun i -> inv i p `star` inames_live ctx)
 
 val new_invariant (e:inames) (p:slprop)
 : ghost_act iref e p (fun i -> inv i p)
+
+val inames_live_inv (e:inames) (i:iref) (p:slprop)
+: ghost_act unit e (inv i p) (fun _ -> inv i p `star` inames_live (single i))
 
 val with_invariant (#a:Type)
                    (#fp:slprop)
